<?xml version="1.0"?>
<rdf:RDF xmlns="https://w3id.org/rec/analytics/"
     xml:base="https://w3id.org/rec/analytics/"
     xmlns:cc="http://creativecommons.org/ns#"
     xmlns:dc="http://purl.org/dc/elements/1.1/"
     xmlns:o2o="https://karlhammar.com/owl2oas/o2o.owl#"
     xmlns:owl="http://www.w3.org/2002/07/owl#"
     xmlns:rdf="http://www.w3.org/1999/02/22-rdf-syntax-ns#"
     xmlns:xml="http://www.w3.org/XML/1998/namespace"
     xmlns:xsd="http://www.w3.org/2001/XMLSchema#"
     xmlns:core="https://w3id.org/rec/core/"
     xmlns:qudt="http://qudt.org/schema/qudt/"
     xmlns:rdfs="http://www.w3.org/2000/01/rdf-schema#"
     xmlns:skos="http://www.w3.org/2004/02/skos/core#"
     xmlns:vaem="http://www.linkedmodel.org/schema/vaem#"
     xmlns:vann="http://purl.org/vocab/vann/"
     xmlns:core1="http://www.linkedmodel.org/owl/schema/core#"
     xmlns:dcterms="http://purl.org/dc/terms/"
     xmlns:opla-sd="http://ontologydesignpatterns.org/opla-sd#"
     xmlns:metadata="https://w3id.org/rec/metadata/"
     xmlns:analytics="https://w3id.org/rec/analytics/"
     xmlns:cpannotationschema="http://www.ontologydesignpatterns.org/schemas/cpannotationschema.owl#">
    <owl:Ontology rdf:about="https://w3id.org/rec/analytics/">
        <owl:versionIRI rdf:resource="https://w3id.org/rec/analytics/3.3/"/>
        <owl:imports rdf:resource="https://w3id.org/rec/core/3.3/"/>
        <cc:license rdf:resource="https://opensource.org/licenses/MIT"/>
        <dc:creator rdf:datatype="http://www.w3.org/2001/XMLSchema#string">Erik Wallin</dc:creator>
        <dc:creator rdf:datatype="http://www.w3.org/2001/XMLSchema#string">Joakim Eriksson</dc:creator>
        <dc:creator rdf:datatype="http://www.w3.org/2001/XMLSchema#string">Karl Hammar</dc:creator>
        <dc:creator rdf:datatype="http://www.w3.org/2001/XMLSchema#string">Per Karlberg</dc:creator>
        <dc:creator rdf:datatype="http://www.w3.org/2001/XMLSchema#string">Peter Hartlev</dc:creator>
        <dc:description xml:lang="en">This RealEstateCore module provides a vocabulary for describing prognoses and aggregates, and the processes used to generate these. This vocabulary is rather generic; we would like to get feedback on it and in particular solicit recommendations on how to model/document anlysis procedures/workflows.</dc:description>
        <dc:publisher>RealEstateCore Consortium</dc:publisher>
        <dc:title>RealEstateCore Analytics Module</dc:title>
        <dcterms:modified rdf:datatype="http://www.w3.org/2001/XMLSchema#string">2020-06-23</dcterms:modified>
        <vann:preferredNamespacePrefix>analytics</vann:preferredNamespacePrefix>
        <vann:preferredNamespaceUri>https://w3id.org/rec/analytics/3.3/</vann:preferredNamespaceUri>
        <rdfs:seeAlso rdf:resource="https://w3id.org/rec/"/>
        <owl:versionInfo rdf:datatype="http://www.w3.org/2001/XMLSchema#string">3.3</owl:versionInfo>
    </owl:Ontology>
    


    <!-- 
    ///////////////////////////////////////////////////////////////////////////////////////
    //
    // Object Properties
    //
    ///////////////////////////////////////////////////////////////////////////////////////
     -->

    


    <!-- https://w3id.org/rec/analytics/analysisConfiguration -->

    <owl:ObjectProperty rdf:about="https://w3id.org/rec/analytics/analysisConfiguration">
        <rdfs:domain rdf:resource="https://w3id.org/rec/analytics/AnalysisProcess"/>
        <rdfs:range rdf:resource="https://w3id.org/rec/analytics/AnalysisConfiguration"/>
        <rdfs:comment xml:lang="en">The configuration for a given analysis process. E.g., which model was used for a machine learning classifier, which dataset was that model trained on, which algorithm was used for some prediction or aggregation, etc. The modelling of specific analysis processes and their semantics remains to be done.</rdfs:comment>
        <rdfs:label xml:lang="en">analysis configuration</rdfs:label>
    </owl:ObjectProperty>
    


    <!-- https://w3id.org/rec/analytics/generatedBy -->

    <owl:ObjectProperty rdf:about="https://w3id.org/rec/analytics/generatedBy">
        <rdfs:subPropertyOf rdf:resource="http://www.w3.org/2002/07/owl#topObjectProperty"/>
        <rdfs:range rdf:resource="https://w3id.org/rec/analytics/AnalysisProcess"/>
        <rdfs:comment xml:lang="en">Links some generated analysis results (predictions, aggregates, series, etc). to the process by which they were created.</rdfs:comment>
        <rdfs:label xml:lang="en">generated by</rdfs:label>
    </owl:ObjectProperty>
    


    <!-- https://w3id.org/rec/analytics/seriesMembers -->

    <owl:ObjectProperty rdf:about="https://w3id.org/rec/analytics/seriesMembers">
        <rdfs:domain rdf:resource="https://w3id.org/rec/analytics/DataSeries"/>
        <rdfs:range rdf:resource="https://w3id.org/rec/core/Observation"/>
        <rdfs:comment xml:lang="en">Members of the data series. Carries the o2o:listProperty annotation, so will in API:s be translated into an RDF ordered list, see https://github.com/RealEstateCore/rec/tree/master/docs/RdfLists.md</rdfs:comment>
        <rdfs:label xml:lang="en">series members</rdfs:label>
        <o2o:listProperty rdf:datatype="http://www.w3.org/2001/XMLSchema#boolean">true</o2o:listProperty>
    </owl:ObjectProperty>
    


    <!-- 
    ///////////////////////////////////////////////////////////////////////////////////////
    //
    // Classes
    //
    ///////////////////////////////////////////////////////////////////////////////////////
     -->

    


    <!-- https://w3id.org/rec/analytics/Aggregate -->

    <owl:Class rdf:about="https://w3id.org/rec/analytics/Aggregate">
        <rdfs:subClassOf rdf:resource="https://w3id.org/rec/core/Observation"/>
        <rdfs:subClassOf>
            <owl:Restriction>
                <owl:onProperty rdf:resource="https://w3id.org/rec/analytics/generatedBy"/>
                <owl:qualifiedCardinality rdf:datatype="http://www.w3.org/2001/XMLSchema#nonNegativeInteger">1</owl:qualifiedCardinality>
                <owl:onClass rdf:resource="https://w3id.org/rec/analytics/AnalysisProcess"/>
            </owl:Restriction>
        </rdfs:subClassOf>
    </owl:Class>
    


    <!-- https://w3id.org/rec/analytics/AnalysisConfiguration -->

    <owl:Class rdf:about="https://w3id.org/rec/analytics/AnalysisConfiguration">
        <rdfs:subClassOf rdf:resource="https://w3id.org/rec/core/Information"/>
        <rdfs:comment xml:lang="en">The configuration for a given analysis process. E.g., which model was used for a machine learning classifier, which dataset was that model trained on, which algorithm was used for some prediction or aggregation, etc. The modelling of specific analysis processes and their semantics remains to be done.</rdfs:comment>
        <rdfs:label xml:lang="en">Analysis configuration</rdfs:label>
    </owl:Class>
    


    <!-- https://w3id.org/rec/analytics/AnalysisProcess -->

    <owl:Class rdf:about="https://w3id.org/rec/analytics/AnalysisProcess">
        <rdfs:comment xml:lang="en">Some process that generates analysis results, e.g., predictions, aggregates, series, etc. This could be anything from the execution of a machine learning classifier to a simple mathematical averaging operation. The modelling of specific analysis processes and their semantics remains to be done.</rdfs:comment>
        <rdfs:label xml:lang="en">Analysis process</rdfs:label>
    </owl:Class>
    


    <!-- https://w3id.org/rec/analytics/DataSeries -->

    <owl:Class rdf:about="https://w3id.org/rec/analytics/DataSeries">
        <rdfs:subClassOf rdf:resource="https://w3id.org/rec/core/Information"/>
        <rdfs:subClassOf>
            <owl:Restriction>
                <owl:onProperty rdf:resource="https://w3id.org/rec/analytics/seriesMembers"/>
                <owl:minQualifiedCardinality rdf:datatype="http://www.w3.org/2001/XMLSchema#nonNegativeInteger">1</owl:minQualifiedCardinality>
                <owl:onClass rdf:resource="https://w3id.org/rec/core/Observation"/>
            </owl:Restriction>
        </rdfs:subClassOf>
        <rdfs:subClassOf>
            <owl:Restriction>
                <owl:onProperty rdf:resource="https://w3id.org/rec/analytics/generatedBy"/>
                <owl:maxQualifiedCardinality rdf:datatype="http://www.w3.org/2001/XMLSchema#nonNegativeInteger">1</owl:maxQualifiedCardinality>
                <owl:onClass rdf:resource="https://w3id.org/rec/analytics/AnalysisProcess"/>
            </owl:Restriction>
        </rdfs:subClassOf>
        <rdfs:comment xml:lang="en">A series of somehow related observations.</rdfs:comment>
        <rdfs:label xml:lang="en">Data series</rdfs:label>
    </owl:Class>
    


    <!-- https://w3id.org/rec/analytics/Prediction -->

    <owl:Class rdf:about="https://w3id.org/rec/analytics/Prediction">
        <rdfs:subClassOf rdf:resource="https://w3id.org/rec/core/Observation"/>
        <rdfs:subClassOf>
            <owl:Restriction>
                <owl:onProperty rdf:resource="https://w3id.org/rec/analytics/generatedBy"/>
                <owl:qualifiedCardinality rdf:datatype="http://www.w3.org/2001/XMLSchema#nonNegativeInteger">1</owl:qualifiedCardinality>
                <owl:onClass rdf:resource="https://w3id.org/rec/analytics/AnalysisProcess"/>
            </owl:Restriction>
        </rdfs:subClassOf>
    </owl:Class>
</rdf:RDF>



<!-- Generated by the OWL API (version 4.5.9.2019-02-01T07:24:44Z) https://github.com/owlcs/owlapi -->

